src/langs/Subst.v
@@ -126,6 +126,169 @@ Definition subst_lang : lang :=
 
 Require Import Setoid.
 
+(* Tactics for easy rule application: todo;
+   move to separate file
+ *)
+
+From Ltac2 Require Import Ltac2.
+(* TODO: generalize over key, value types? *)
+Ltac2 Type rec FinMap :=
+  [ MapEmpty
+  | MapCons (int, constr, FinMap)].
+
+Ltac2 Type exn ::= [EmptyMapLookupExn].
+Ltac2 rec map_lookup n m :=
+  match m with
+  | MapEmpty => Control.zero EmptyMapLookupExn
+  | MapCons n' v m' =>
+    match Int.equal n' n with
+    | true => v
+    | false => map_lookup n m'
+    end
+  end.
+
+(* Computes a map that has all mappings from both,
+   or throws if none exists
+TODO: optimize representation for this operation
+ *)
+Ltac2 Type exn ::= [MapMergeExn(constr, constr)].
+Ltac2 rec map_merge m1 m2 :=
+  match m1 with
+  | MapEmpty => m2
+  | MapCons k v1 m1' =>
+    MapCons k v1
+            (Control.plus
+               (fun _ => let v2 := map_lookup k m2 in
+                match Constr.equal v1 v2 with
+                | true => map_merge m1' m2
+                | false => Control.zero (MapMergeExn v1 v2)
+                end)
+               (fun ex =>
+                  match ex with
+                  | EmptyMapLookupExn => map_merge m1' m2
+                  | _ => Control.zero ex
+                  end))
+  end.
+
+Ltac2 Type exn ::= [DomainExn(constr, constr, constr)].
+Ltac2 dom_exn c t := DomainExn c (Constr.type c) t.
+Ltac2 rec int_of_nat c :=
+  match! c with
+  | 0 => 0
+  | S ?c' => Int.add 1 (int_of_nat c')
+  | _ => Control.throw (dom_exn c constr:(nat)) 
+  end.
+
+Ltac2 Type exn ::= [ExpMatchExn(constr, constr)].
+Ltac2 rec exp_match (p : constr) e :=
+  match! p with
+  | var ?x => MapCons (int_of_nat x) e MapEmpty
+  | con ?pn ?ps =>
+    match! e with
+    | con ?n ?s =>
+      match Constr.equal pn n with
+      | true => subst_match ps s
+      | false => Control.throw (ExpMatchExn p e)
+      end
+    | var _ => Control.throw (ExpMatchExn p e)
+    | _ => Control.throw (dom_exn e constr:(exp))
+      (* TODO: need to handle evars*)
+    end
+  | _ => Control.throw (dom_exn p constr:(exp))
+  end
+with subst_match p s :=
+    match! p with
+    | [::] => match! s with [::] => MapEmpty end
+    | ?pe::?p' =>
+      match! s with
+      | ?e::?s' =>
+        map_merge (exp_match pe e) (subst_match p' s')
+      | [::] => Control.throw (ExpMatchExn p s)
+      end
+    end.
+
+Ltac2 Eval (exp_match constr:(var 1) constr:(var 2)).
+Ltac2 Eval
+      (exp_match constr:(con 1 [:: var 2; var 2])
+                          constr:(con 1 [:: (con 2 [::]); (con 2 [::])])).
+
+
+(* assumes idx <= size 
+   TODO: how to handle terms that aren't listed?
+   evar?
+*)
+Ltac2 subst_of_map m size :=
+  let rec som idx acc :=
+      match Int.equal idx size with
+      | true => acc
+      | false =>
+        let v := map_lookup idx m in
+        som (Int.add idx 1) constr:($v::$acc)
+      end in
+  som 0 constr:(@nil exp).
+
+Ltac2 Eval (subst_of_map
+              (MapCons 2 constr:(var 3)
+              (MapCons 0 constr:(var 1)
+              (MapCons 1 constr:(var 2) MapEmpty)))) 3.
+
+Ltac2 max n m :=
+  match Int.gt n m with
+  | true => n
+  | false => m
+  end.
+
+Ltac2 rec min_subst_size m :=
+  match m with
+  | MapEmpty => 0
+  | MapCons n _ m' =>
+    max (Int.add n 1) (min_subst_size m')
+  end.
+
+(* taken from https://github.com/coq/coq/issues/11641 *)
+Ltac2 my_change2 (a : constr) (b : constr) :=
+  ltac1:( a b |- change a with b ) (Ltac1.of_constr a) (Ltac1.of_constr b).
+
+Require Import Ltac2.Notations.
+
+Ltac2 rec unify_in () :=
+  match! goal with
+    [|- is_true (?r \in ?r'::?l)] =>
+    rewrite in_cons;
+    ltac1:(apply /orP);
+    Control.plus
+      (fun () => left;ltac1:(apply /eqP; by f_equal))
+      (fun _ =>
+         right; unify_in ())
+end.
+
+Ltac2 apply_term_rule n :=
+  match! goal with
+    [|- le_term ?l ?c ?t ?e1 ?e2 ]=>
+    match! Std.eval_hnf constr:(nth_level (sort_rule [::]) $l $n) with
+      term_le _ ?pe1 ?pe2 ?pt =>
+      let m := subst_match constr:([:: $pt; $pe1; $pe2])
+                           constr:([:: $t; $e1; $e2]) in
+      let s := subst_of_map m (min_subst_size m) in
+      my_change2
+        constr:(le_term $l $c $t $e1 $e2)
+        constr:(le_term $l $c $pt[/$s/] $pe1[/$s/] $pe2[/$s/]);
+      eapply le_term_subst;
+      Control.enter
+        (fun () =>
+           match! goal with
+           | [|- le_term _ _ _ _ _] =>
+             eapply le_term_by;
+             unify_in ()
+           | [|- le_subst _ _ _ _ _] => ()
+           | [|- _] => Control.throw Match_failure
+           end)
+    end
+  end.
+
+
+
+Set Default Proof Mode "Classic".
 Lemma subst_lang_wf : wf_lang subst_lang.
 Proof using .
   wf_lang_eauto.
@@ -146,7 +309,8 @@ Proof using .
 
     eapply sort_con_mor.
     eapply subst_cons_mor.
-    eapply reflexivity.
+    eapply subst_cons_mor; try reflexivity.
+    eauto with judgment.
     change ( [:: el 0 1; ty 0; ob] ) with ( [:: el 0 1]++[:: ty 0; ob] ).
     eapply le_mono_ctx.
     eapply le_term_by.
@@ -164,28 +328,29 @@ Proof using .
     auto with judgment.
     auto with judgment.
     
-    (*TODO: eapply symmetry does something very bad; why?*)
-    match goal with |- le_term ?l ?c _ _ ?t => eapply (@symmetry _ (fun x y => le_term l c x y t)) end.
-    eauto with typeclass_instances.
-    (* TODO: why doesn't this work? setoid_symmetry relation (fun x y => le_term l c x y t).*)
     eapply le_term_trans.
-    2:{
-    match goal with |- le_term ?l ?c _ _ ?t => eapply (@symmetry _ (fun x y => le_term l c x y t)) end.
-    eauto with typeclass_instances.
-    
-    match goal with _ : wf_lang ?l |- _ => let e := eval cbv in (size l) in idtac e end.
-    
-    setoid_replace (ty_subst 0 (ext 1 3) (snoc 0 1 3 2 4) (ty_subst (ext 1 3) 1 (p 1 3) 3))
-                   with (ty_subst 0 1 (cmp 0 (ext 1 3) 1 (p 1 3) (snoc 0 1 3 2 4)) 3).
-    match goal with
-      |- le_term _ _ 
-    strategy: rewrite to compose, compose p with snoc
-    TODO: add symmetric rules to fuller framework.
-
-    instantiate
-      (1:= (el 0 (ty_subst 0 1 2
-                           (ty_subst (ext 1 3) 1 (p 1 3) 3)))).
-    apply:type_wf_term_recognizes; eauto with judgment.
-    compute.
+    instantiate (2 := ty 0); cbv.
+    - symmetry (* TODO: handle in tactic *).
+      instantiate (1 := ty_subst 0 1
+                           (cmp 0 (ext 1 3) 1
+                                (p 1 3) (snoc 0 1 3 2 4))
+                           3)
+      (*TODO: handle in tactic*).
+      ltac2:(apply_term_rule constr:(14)).
+      eauto with judgment.
+    -
+      (* TODO: should be handled by tactic *)
+      change (ty 0)[/[:: var 0]/]
+        with (ty 0)[/[:: var 3; var 2; var 1; var 0]/].
+      eapply term_con_mor.
+      repeat eapply subst_cons_mor;
+        auto with judgment.
+      instantiate (1:= hom 0 1).
+      cbv.
+      ltac2:(apply_term_rule constr:(23)).
+      eauto with judgment.
+      Unshelve.
+      all: try exact (con 0 [::]).
+      all: exact [::].
+  }
 Qed.
-es
